theories/Weakening.v
@@ -6,29 +6,256 @@ Require Import Behavior.
 Require Import ModSem.
 Require Import Skeleton.
 Require Import PCM.
-Require Import Hoare.
+Require Import HoareDef.
 Require Import SimModSem.
 
 Require Import HTactics.
 
-Generalizable Variables E R A B C X Y Σ.
+From ITree Require Import
+     Events.MapDefault.
+From ExtLib Require Import
+     Core.RelDec
+     Structures.Maps
+     Data.Map.FMapAList.
 
 Set Implicit Arguments.
 
 
 
 
-Definition ord_le (next cur: ord): Prop :=
-  match next, cur with
-  | ord_pure next, ord_pure cur => (next <= cur)%nat
-  | _, ord_top => True
-  | _, _ => False
-  end
-.
 
 Section PROOF.
 
   Context `{Σ: GRA.t}.
+
+  Let W: Type := (alist mname (Σ * Any.t)) * (alist mname (Σ * Any.t)).
+
+
+(*   Variant bindR (r s:  *)
+
+(*           (r s: forall S (SS: S -> S -> Prop), Ordinal.t -> (itree eventE S) -> (itree eventE S) -> Prop): *)
+(*     forall S (SS: S -> S -> Prop), Ordinal.t -> (itree eventE S) -> (itree eventE S) -> Prop := *)
+(*   | bindR_intro *)
+(*       o0 o1 *)
+
+(*       R RR *)
+(*       (i_src i_tgt: itree eventE R) *)
+(*       (SIM: r _ RR o0 i_src i_tgt) *)
+
+(*       S SS *)
+(*       (k_src k_tgt: ktree eventE R S) *)
+(*       (SIMK: forall vret_src vret_tgt (SIM: RR vret_src vret_tgt), s _ SS o1 (k_src vret_src) (k_tgt vret_tgt)) *)
+(*     : *)
+(*       bindR r s SS (Ordinal.add o1 o0) (ITree.bind i_src k_src) (ITree.bind i_tgt k_tgt) *)
+(*   . *)
+
+(* _sim_itree *)
+
+(* _sim_itree *)
+(*      : (FMapAList.alist string (Σ * Any.t) * FMapAList.alist string (Σ * Any.t) -> *)
+(*         Prop) -> *)
+(*        (nat -> *)
+(*         Relation_Definitions.relation *)
+(*           (FMapAList.alist string (Σ * Any.t) * Σ * itree Es Any.t)) -> *)
+(*        nat -> *)
+(*        Relation_Definitions.relation *)
+(*          (FMapAList.alist string (Σ * Any.t) * Σ * itree Es Any.t) *)
+
+
+(* Hint Constructors bindR: core. *)
+
+(* Lemma bindR_mon *)
+(*       r1 r2 s1 s2 *)
+(*       (LEr: r1 <5= r2) (LEs: s1 <5= s2) *)
+(*   : *)
+(*     bindR r1 s1 <5= bindR r2 s2 *)
+(* . *)
+(* Proof. ii. destruct PR; econs; et. Qed. *)
+
+(* Definition bindC r := bindR r r. *)
+(* Hint Unfold bindC: core. *)
+
+(* Lemma bindC_wrespectful: wrespectful5 (_simg) bindC. *)
+(* Proof. *)
+(*   econstructor; repeat intro. *)
+(*   { eapply bindR_mon; eauto. } *)
+(*   rename l into llll. *)
+(*   eapply bindR_mon in PR; cycle 1. *)
+(*   { eapply GF. } *)
+(*   { i. eapply PR0. } *)
+(*   inv PR. csc. inv SIM. *)
+(*   + irw. *)
+(*     exploit SIMK; eauto. i. *)
+(*     eapply simg_mon_ord. *)
+(*     { instantiate (1:=o1). eapply Ordinal.add_base_l. } *)
+(*     eapply simg_mon; eauto with paco. *)
+(*   + rewrite ! bind_bind. econs; eauto. ii. *)
+(*     { econs 2; eauto with paco. econs; eauto with paco. } *)
+
+
+(*   + irw. econs; eauto. *)
+(*     (* { eapply Ordinal.add_le_r; et. } *) *)
+(*     { econs 2; eauto with paco. econs; eauto with paco. } *)
+(*   + rewrite ! bind_tau. econs; eauto. *)
+(*     { instantiate (1:= Ordinal.add o1 i1). eapply Ordinal.add_lt_r; et. } *)
+(*     econs 2; eauto with paco. econs; eauto with paco. *)
+(*   + irw. econs; eauto. *)
+(*     { instantiate (1:= Ordinal.add o1 i1). eapply Ordinal.add_lt_r; et. } *)
+(*     econs 2; eauto with paco. econs; eauto with paco. *)
+
+
+(*   + rewrite ! bind_bind. econs; eauto. *)
+(*     (* { eapply Ordinal.add_le_r; et. } *) *)
+(*     { ii. spc SIM0. des. esplits; et. econs 2; eauto with paco. econs; eauto with paco. } *)
+(*   + rewrite ! bind_bind. econs; eauto. *)
+(*     { instantiate (1:= Ordinal.add o1 i1). eapply Ordinal.add_lt_r; et. } *)
+(*     des. esplits; et. econs 2; eauto with paco. econs; eauto with paco. *)
+(*   + rewrite ! bind_bind. econs; eauto. *)
+(*     { instantiate (1:= Ordinal.add o1 i1). eapply Ordinal.add_lt_r; et. } *)
+(*     des. esplits; et. econs 2; eauto with paco. econs; eauto with paco. *)
+
+(*   + rewrite ! bind_bind. econs; eauto. *)
+(*     (* { eapply Ordinal.add_le_r; et. } *) *)
+(*     { ii. spc SIM0. des. esplits; et. econs 2; eauto with paco. econs; eauto with paco. } *)
+(*   + rewrite ! bind_bind. econs; eauto. *)
+(*     { instantiate (1:= Ordinal.add o1 i1). eapply Ordinal.add_lt_r; et. } *)
+(*     des. esplits; et. econs 2; eauto with paco. econs; eauto with paco. *)
+(*   + rewrite ! bind_bind. econs; eauto. *)
+(*     { instantiate (1:= Ordinal.add o1 i1). eapply Ordinal.add_lt_r; et. } *)
+(*     des. esplits; et. econs 2; eauto with paco. econs; eauto with paco. *)
+(* Qed. *)
+
+
+  Variant fspec_weaker (fsp_src fsp_tgt: fspec): Prop :=
+  | fspec_weaker_intro
+      mn X_src X_tgt AA AR P_src P_tgt Q_src Q_tgt
+      (FSPEC0: fsp_src = @mk _ mn X_src AA AR P_src Q_src)
+      (FSPEC1: fsp_tgt = @mk _ mn X_tgt AA AR P_tgt Q_tgt)
+      (WEAK: forall (x_src: X_src),
+          exists (x_tgt: X_tgt),
+            (<<PRE: P_tgt x_tgt <4= P_src x_src>>) /\
+            (<<POST: Q_src x_src <3= Q_tgt x_tgt>>))
+  .
+
+  Variable stb_src stb_tgt: list (gname * fspec).
+  Hypothesis stb_stronger:
+    forall fn fn_tgt fsp_tgt (FINDTGT: List.find (fun '(_fn, _) => dec fn _fn) stb_tgt = Some (fn_tgt, fsp_tgt)),
+    exists fn_src fsp_src,
+      (<<FINDSRC: List.find (fun '(_fn, _) => dec fn _fn) stb_src = Some (fn_src, fsp_src)>>) /\
+      (<<WEAKER: fspec_weaker fsp_tgt fsp_src>>)
+  .
+
+  Variable fn: gname.
+
+  Variable fsp_src fsp_tgt: fspec.
+  Hypothesis fsp_weaker: fspec_weaker fsp_src fsp_tgt.
+
+  Variable body_src: fsp_src.(AA) -> itree (hCallE +' pE +' eventE) fsp_src.(AR).
+  Variable body_tgt: fsp_tgt.(AA) -> itree (hCallE +' pE +' eventE) fsp_tgt.(AR).
+  Hypothesis body_eq: JMeq body_src body_tgt.
+
+  Lemma weakening_fn:
+    sim_fsem (fun '(w_src, w_tgt) => w_src = w_tgt)
+             (fun_to_tgt stb_src fn (mk_specbody fsp_src body_src))
+             (fun_to_tgt stb_tgt fn (mk_specbody fsp_tgt body_tgt)).
+  Proof.
+    inv fsp_weaker. ss. subst. ii. subst. exists 0.
+    unfold fun_to_tgt. ss. repeat rewrite HoareFun_parse.
+
+    ginit.
+
+    ii. subst. exists 0. unfold funOt
+
+
+
+
+    (mk_specbody fsp_src body_tgt))
+
+
+  (AR fsb_fspe)c
+
+    :=
+
+
+  fspecbody
+
+  Variable body: AA fsb_fspec -> itree (hCallE +' pE +' eventE) (AR fsb_fspec).
+
+  sim_fsem
+
+
+
+
+         forall fn x (FINDSRC: List.find (fun '(_fn, _) => dec fn _fn) stb_src = Some (fn_src, fsp_src))
+      exists fn_tgt fsp_tgt,
+        (<<FINDTGT: List.find (fun '(_fn, _) => dec fn _fn) stb_tgt = x.
+
+  Lemma sim_fnsem_wf fn
+
+
+
+  Definition Fsbtb: list (string * fspecbody) := [("f", mk_specbody f_spec (fun _ => trigger (Choose _)))].
+
+  Definition FSem: ModSem.t := {|
+    ModSem.fnsems := List.map (fun '(fn, body) => (fn, fun_to_tgt GlobalStb fn body)) Fsbtb;
+    ModSem.initial_mrs := [("F", (ε, tt↑))];
+  |}
+  .
+
+  Record fspecbody (Σ : GRA.t) : Type := mk_specbody
+  { fsb_fspec : fspec;
+    fsb_body : AA fsb_fspec -> itree (hCallE +' pE +' eventE) (AR fsb_fspec) }
+
+
+        fun_to_tgt GlobalStb fn body
+
+  sim_fnsem wf
+
+  fspec_
+
+  /\
+
+
+
+                    (a_src: AA_src) (r_src: AR_src) (o_src: ord)
+                    (PRE: P_src x_src a_src
+                                exists (x_tgt: X_tgt) (a_tgt: AA_tgt) (r_tgt: AR_tgt) (o_tgt: ord)
+
+
+
+.
+  Variant fspec_weaker (fsp_src fsp_tgt: fspec): Prop :=
+  | fspec_weaker_intro
+      mn X_src X_tgt AA_src AA_tgt AR_src AR_tgt
+      P_src P_tgt Q_src Q_tgt
+      (FSPEC0: fsp_src = @mk _ mn X_src AA_src AR_src P_src Q_src)
+      (FSPEC1: fsp_tgt = @mk _ mn X_tgt AA_tgt AR_tgt P_tgt Q_tgt)
+      (WEAK: forall (x_src: X_src),
+          exists (x_tgt: X_tgt),
+            (<<PRE: forall arg varg_src o_src rarg_src
+                           (PRE: P_src x_src varg_src arg o_src rarg_src),
+                exists varg_tgt o_tgt rarg_tgt,
+                  (<<PRE: P_tgt x_tgt varg_tgt arg o_tgt rarg_tgt>>) /\
+
+
+                (a_src: AA_src) (r_src: AR_src) (o_src: ord)
+                    (PRE: P_src x_src a_src
+                            exists (x_tgt: X_tgt) (a_tgt: AA_tgt) (r_tgt: AR_tgt) (o_tgt: ord)
+
+
+  Variant fspec_weaker (fsp_src fsp_tgt: fspec): Prop :=
+  | fspec_weaker_intro
+      mn X AA AR P_src P_tgt Q_src Q_tgt
+      (FSPEC0: fsp_src = @mk _ mn X AA AR P_src Q_src)
+      (FSPEC1: fsp_tgt = @mk _ mn X AA AR P_tgt Q_tgt)
+      (WEAK: forall x aarg rarg
+
+          (x_src: X_src) (a_src: AA_src) (r_src: AR_src) (o_src: ord)
+                    (PRE: P_src x_src a_src
+                                exists (x_tgt: X_tgt) (a_tgt: AA_tgt) (r_tgt: AR_tgt) (o_tgt: ord)
+
+
+       .
 
   Variant fspec_weaker (fsp_src fsp_tgt: fspec): Prop :=
   | fspec_weaker_intro
@@ -36,7 +263,14 @@ Section PROOF.
       P_src P_tgt Q_src Q_tgt
       (FSPEC0: fsp_src = @mk _ mn X_src AA_src AR_src P_src Q_src)
       (FSPEC1: fsp_tgt = @mk _ mn X_tgt AA_tgt AR_tgt P_tgt Q_tgt)
-  .
+      (WEAK: forall (x_src: X_src) (a_src: AA_src) (r_src: AR_src) (o_src: ord)
+                    (PRE: P_src x_src a_src
+                            exists (x_tgt: X_tgt) (a_tgt: AA_tgt) (r_tgt: AR_tgt) (o_tgt: ord)
+
+
+       .
+
+fspec
 
 Lemma
 
